preservation.lean
@@ -32,71 +32,291 @@ lemma same_calls_and_left {P P' Q: prop} {σ: env}:
   set.eq_of_subset_of_subset (
     assume c: calltrigger,
     assume : c ∈ calls_env σ (P' ⋀ Q),
-    or.elim (has_call_env.and.inv this) (
+    or.elim (prop.has_call_env.and.inv this) (
       assume : c ∈ calls_env σ P',
       have c ∈ calls_env σ P, from calls_P'_P ▸ this,
-      show c ∈ calls_env σ (P ⋀ Q), from has_call_env.and₁ this
+      show c ∈ calls_env σ (P ⋀ Q), from prop.has_call_env.and₁ this
     )
     (
       assume : c ∈ calls_env σ Q,
-      show c ∈ calls_env σ (P ⋀ Q), from has_call_env.and₂ this
+      show c ∈ calls_env σ (P ⋀ Q), from prop.has_call_env.and₂ this
     )
   )
   (
     assume c: calltrigger,
     assume : c ∈ calls_env σ (P ⋀ Q),
-    or.elim (has_call_env.and.inv this) (
+    or.elim (prop.has_call_env.and.inv this) (
       assume : c ∈ calls_env σ P,
       have c ∈ calls_env σ P', from calls_P'_P.symm ▸ this,
-      show c ∈ calls_env σ (P' ⋀ Q), from has_call_env.and₁ this
+      show c ∈ calls_env σ (P' ⋀ Q), from prop.has_call_env.and₁ this
     )
     (
       assume : c ∈ calls_env σ Q,
-      show c ∈ calls_env σ (P' ⋀ Q), from has_call_env.and₂ this
+      show c ∈ calls_env σ (P' ⋀ Q), from prop.has_call_env.and₂ this
     )
   )
 
-lemma same_quantifiers_and_left {P P' Q: prop} {σ: env}:
-      qualifiers_dominate σ P' P → qualifiers_dominate σ (P' ⋀ Q) (P ⋀ Q) :=
-  assume P'_dominates_P: qualifiers_dominate σ P' P,
-  assume (t₁: term) (x:var) (Q₁: prop),
-  assume : callquantifier.mk t₁ x Q₁ ∈ quantifiers (P ⋀ Q),
-  or.elim (has_quantifier.and.inv this) (
-    assume : callquantifier.mk t₁ x Q₁ ∈ quantifiers P,
-    have ∃(t₂: term) (Q₂: prop), callquantifier.mk t₂ x Q₂ ∈ quantifiers P' ∧
-        ∀v: value, σ[x↦v] ⊨ vc.implies Q₂.instantiated Q₁.instantiated,
-    from P'_dominates_P t₁ x Q₁ this,
-    let ⟨t₂, Q₂, ⟨call_t₂_Q₂_in_P', Q₂_impl_Q₁⟩⟩ := this in
-    have callquantifier.mk t₂ x Q₂ ∈ quantifiers (P' ⋀ Q), from has_quantifier.and₁ call_t₂_Q₂_in_P',
-    show ∃(t₂: term) (Q₂: prop), callquantifier.mk t₂ x Q₂ ∈ quantifiers (P' ⋀ Q) ∧
-        ∀v: value, σ[x↦v] ⊨ vc.implies Q₂.instantiated Q₁.instantiated,
-    from exists.intro t₂ (exists.intro Q₂ ⟨this, Q₂_impl_Q₁⟩)
-  ) (
-    assume : callquantifier.mk t₁ x Q₁ ∈ quantifiers Q,
-    have h1: callquantifier.mk t₁ x Q₁ ∈ quantifiers (P' ⋀ Q), from has_quantifier.and₂ this,
-    have h2: ∀v: value, σ[x↦v] ⊨ vc.implies Q₁.instantiated Q₁.instantiated, from (
+lemma dominates_self: ∀ {P: prop} {σ: env}, dominates σ P P
+| P σ :=
+  have h_impl: σ ⊨ vc.implies P.instantiated_n P.instantiated_n, from valid_env.mpr id,
+  have h_calls: calls_env σ P = calls_env σ P, from rfl,
+  have h_quantifiers:
+    (∀(t': term) (x: var) (Q₁: prop) (h: callquantifier.mk t' x Q₁ ∈ quantifiers P),
+                          have Q₁.size < P.size, from quantifiers_smaller_than_prop.left h,
+    ∃(t: term) (Q₂: prop), callquantifier.mk t x Q₂ ∈ quantifiers P ∧
+                          (∀v: value, dominates' Q₁ Q₂ (σ[x↦v]))), from (
+    assume (t₁: term) (x:var) (Q₁: prop),
+    assume h: callquantifier.mk t₁ x Q₁ ∈ quantifiers P,
+    have Q₁.size < P.size, from quantifiers_smaller_than_prop.left h,
+    have (∀v: value, dominates' Q₁ Q₁ (σ[x↦v])), from (
       assume v: value,
-      show σ[x↦v] ⊨ vc.implies Q₁.instantiated Q₁.instantiated, from valid_env.mpr id
+      dominates_self
     ),
-    show ∃(t₂: term) (Q₂: prop), callquantifier.mk t₂ x Q₂ ∈ quantifiers (P' ⋀ Q) ∧
-        ∀v: value, σ[x↦v] ⊨ vc.implies Q₂.instantiated Q₁.instantiated,
-    from exists.intro t₁ (exists.intro Q₁ ⟨h1, h2⟩)
+    exists.intro t₁ (exists.intro Q₁ ⟨h, this⟩)
+  ),
+  have h3: 
+    ((σ ⊨ vc.implies P.instantiated_n P.instantiated_n) ∧
+    (calls_env σ P = calls_env σ P) ∧
+    (∀(t': term) (x: var) (Q': prop) (h: callquantifier.mk t' x Q' ∈ quantifiers P),
+                          have Q'.size < P.size, from quantifiers_smaller_than_prop.left h,
+    ∃(t: term) (Q₂: prop), callquantifier.mk t x Q₂ ∈ quantifiers P ∧
+                          (∀v: value, dominates' Q' Q₂ (σ[x↦v])))),
+  from ⟨h_impl, ⟨h_calls, h_quantifiers⟩⟩,
+  have
+    dominates' P P σ = (
+    ((σ ⊨ vc.implies P.instantiated_n P.instantiated_n) ∧
+    (calls_env σ P = calls_env σ P) ∧
+    (∀(t': term) (x: var) (Q': prop) (h: callquantifier.mk t' x Q' ∈ quantifiers P),
+                          have Q'.size < P.size, from quantifiers_smaller_than_prop.left h,
+    ∃(t: term) (Q₂: prop), callquantifier.mk t x Q₂ ∈ quantifiers P ∧
+                          (∀v: value, dominates' Q' Q₂ (σ[x↦v]))))),
+  by unfold1 dominates',
+  have dominates' P P σ, from this.symm ▸ h3,
+  show dominates σ P P, from this
+
+lemma dominates_and_left {P P' Q: prop} {σ: env}:
+      dominates σ P' P → dominates σ (P' ⋀ Q) (P ⋀ Q) :=
+  assume h1: dominates σ P' P,
+  have dominates' P P' σ, from h1,
+  have h2:
+    ((σ ⊨ vc.implies P'.instantiated_n P.instantiated_n) ∧
+    (calls_env σ P' = calls_env σ P) ∧
+    (∀(t': term) (x: var) (Q': prop) (h: callquantifier.mk t' x Q' ∈ quantifiers P),
+                          have Q'.size < P.size, from quantifiers_smaller_than_prop.left h,
+    ∃(t: term) (Q: prop), callquantifier.mk t x Q ∈ quantifiers P' ∧
+                          (∀v: value, dominates' Q' Q (σ[x↦v])))),
+  by { unfold1 dominates' at this, from this },
+
+  have calls_env σ P' = calls_env σ P, from h2.right.left,
+  have h_calls: calls_env σ (P' ⋀ Q) = calls_env σ (P ⋀ Q), from same_calls_and_left this,
+  have h_quantifiers:
+    (∀(t': term) (x: var) (Q₁: prop) (h: callquantifier.mk t' x Q₁ ∈ quantifiers (P ⋀ Q)),
+                          have Q₁.size < (P ⋀ Q).size, from quantifiers_smaller_than_prop.left h,
+    ∃(t: term) (Q₂: prop), callquantifier.mk t x Q₂ ∈ quantifiers (P' ⋀ Q) ∧
+                          (∀v: value, dominates' Q₁ Q₂ (σ[x↦v]))), from (
+
+    assume (t₁: term) (x:var) (Q₁: prop),
+    assume : callquantifier.mk t₁ x Q₁ ∈ quantifiers (P ⋀ Q),
+    or.elim (prop.has_quantifier.and.inv this) (
+      assume : callquantifier.mk t₁ x Q₁ ∈ quantifiers P,
+      have ∃(t₂: term) (Q₂: prop), callquantifier.mk t₂ x Q₂ ∈ quantifiers P' ∧
+                          (∀v: value, dominates' Q₁ Q₂ (σ[x↦v])),
+      from h2.right.right t₁ x Q₁ this,
+      let ⟨t₂, Q₂, ⟨call_t₂_Q₂_in_P', Q₂_impl_Q₁⟩⟩ := this in
+      have callquantifier.mk t₂ x Q₂ ∈ quantifiers (P' ⋀ Q), from prop.has_quantifier.and₁ call_t₂_Q₂_in_P',
+      show ∃(t₂: term) (Q₂: prop), callquantifier.mk t₂ x Q₂ ∈ quantifiers (P' ⋀ Q) ∧
+                                   (∀v: value, dominates' Q₁ Q₂ (σ[x↦v])),
+      from exists.intro t₂ (exists.intro Q₂ ⟨this, Q₂_impl_Q₁⟩)
+    ) (
+      assume : callquantifier.mk t₁ x Q₁ ∈ quantifiers Q,
+      have h1: callquantifier.mk t₁ x Q₁ ∈ quantifiers (P' ⋀ Q), from prop.has_quantifier.and₂ this,
+      have h2: ∀v: value, dominates' Q₁ Q₁ (σ[x↦v]), from (
+        assume v: value,
+        show dominates' Q₁ Q₁ (σ[x↦v]), from dominates_self
+      ),
+      show ∃(t₂: term) (Q₂: prop), callquantifier.mk t₂ x Q₂ ∈ quantifiers (P' ⋀ Q) ∧
+                                   (∀v: value, dominates' Q₁ Q₂ (σ[x↦v])),
+      from exists.intro t₁ (exists.intro Q₁ ⟨h1, h2⟩)
+    )
+  ),
+
+  have σ ⊨ vc.implies P'.instantiated_n P.instantiated_n, from h2.left,
+  have h_impl: σ ⊨ vc.implies (P' ⋀ Q).instantiated_n (P ⋀ Q).instantiated_n,
+  from valid_env.strengthen_and_with_dominating_instantiations h1,
+
+  have h3: 
+    ((σ ⊨ vc.implies (P' ⋀ Q).instantiated_n (P ⋀ Q).instantiated_n) ∧
+    (calls_env σ (P' ⋀ Q) = calls_env σ (P ⋀ Q)) ∧
+    (∀(t': term) (x: var) (Q': prop) (h: callquantifier.mk t' x Q' ∈ quantifiers (P ⋀ Q)),
+                          have Q'.size < (P ⋀ Q).size, from quantifiers_smaller_than_prop.left h,
+    ∃(t: term) (Q₂: prop), callquantifier.mk t x Q₂ ∈ quantifiers (P' ⋀ Q) ∧
+                          (∀v: value, dominates' Q' Q₂ (σ[x↦v])))),
+  from ⟨h_impl, ⟨h_calls, h_quantifiers⟩⟩,
+  have
+    dominates' (P ⋀ Q) (P' ⋀ Q) σ = (
+    ((σ ⊨ vc.implies (P' ⋀ Q).instantiated_n (P ⋀ Q).instantiated_n) ∧
+    (calls_env σ (P' ⋀ Q) = calls_env σ (P ⋀ Q)) ∧
+    (∀(t': term) (x: var) (Q': prop) (h: callquantifier.mk t' x Q' ∈ quantifiers (P ⋀ Q)),
+                          have Q'.size < (P ⋀ Q).size, from quantifiers_smaller_than_prop.left h,
+    ∃(t: term) (Q₂: prop), callquantifier.mk t x Q₂ ∈ quantifiers (P' ⋀ Q) ∧
+                          (∀v: value, dominates' Q' Q₂ (σ[x↦v]))))),
+  by unfold1 dominates',
+  have dominates' (P ⋀ Q) (P' ⋀ Q) σ, from this.symm ▸ h3,
+  show dominates σ (P' ⋀ Q) (P ⋀ Q), from this
+
+lemma dominates_not_not: ∀ {P: prop} {σ: env}, dominates σ P.not.not P
+| P σ :=
+  have h_impl: σ ⊨ vc.implies P.not.not.instantiated_n P.instantiated_n, from valid_env.mpr (
+    assume h1: σ ⊨ P.not.not.instantiated_n,
+    have P.not.not.instantiated_n = P.not.instantiated.not, from not_dist_instantiated_n,
+    have h2: σ ⊨ P.not.instantiated.not, from this ▸ h1,
+    have P.not.instantiated = P.instantiated_n.not, from not_dist_instantiated,
+    have σ ⊨ P.instantiated_n.not.not, from this ▸ h2,
+    show σ ⊨ P.instantiated_n, from valid_env.neg_neg.mp this
+  ),
+  have h_calls: calls_env σ P.not.not = calls_env σ P, from set.eq_of_subset_of_subset (
+    assume c: calltrigger,
+    assume : c ∈ calls_env σ P.not.not,
+    have c ∈ calls_n_env σ P.not, from prop.has_call_env.not.inv this,
+    show c ∈ calls_env σ P, from prop.has_call_n_env.not.inv this
+  )
+  (
+    assume c: calltrigger,
+    assume : c ∈ calls_env σ P,
+    have c ∈ calls_n_env σ P.not, from prop.has_call_env.not this,
+    show c ∈ calls_env σ P.not.not, from prop.has_call_n_env.not this
+  ),
+  have h_quantifiers:
+    (∀(t': term) (x: var) (Q₁: prop) (h: callquantifier.mk t' x Q₁ ∈ quantifiers P),
+                          have Q₁.size < P.size, from quantifiers_smaller_than_prop.left h,
+    ∃(t: term) (Q₂: prop), callquantifier.mk t x Q₂ ∈ quantifiers P.not.not ∧
+                          (∀v: value, dominates' Q₁ Q₂ (σ[x↦v]))), from (
+    assume (t₁: term) (x:var) (Q₁: prop),
+    assume h: callquantifier.mk t₁ x Q₁ ∈ quantifiers P,
+    have callquantifier.mk t₁ x Q₁ ∈ quantifiers_n P.not, from prop.has_quantifier_n.not h,
+    have h2: callquantifier.mk t₁ x Q₁ ∈ quantifiers P.not.not, from prop.has_quantifier.not this,
+    have Q₁.size < P.size, from quantifiers_smaller_than_prop.left h,
+    have (∀v: value, dominates' Q₁ Q₁ (σ[x↦v])), from (
+      assume v: value,
+      dominates_self
+    ),
+    exists.intro t₁ (exists.intro Q₁ ⟨h2, this⟩)
+  ),
+  have h3: 
+    ((σ ⊨ vc.implies P.not.not.instantiated_n P.instantiated_n) ∧
+    (calls_env σ P.not.not = calls_env σ P) ∧
+    (∀(t': term) (x: var) (Q': prop) (h: callquantifier.mk t' x Q' ∈ quantifiers P),
+                          have Q'.size < P.size, from quantifiers_smaller_than_prop.left h,
+    ∃(t: term) (Q₂: prop), callquantifier.mk t x Q₂ ∈ quantifiers P.not.not ∧
+                          (∀v: value, dominates' Q' Q₂ (σ[x↦v])))),
+  from ⟨h_impl, ⟨h_calls, h_quantifiers⟩⟩,
+  have
+    dominates' P P.not.not σ = (
+    ((σ ⊨ vc.implies P.not.not.instantiated_n P.instantiated_n) ∧
+    (calls_env σ P.not.not = calls_env σ P) ∧
+    (∀(t': term) (x: var) (Q': prop) (h: callquantifier.mk t' x Q' ∈ quantifiers P),
+                          have Q'.size < P.size, from quantifiers_smaller_than_prop.left h,
+    ∃(t: term) (Q₂: prop), callquantifier.mk t x Q₂ ∈ quantifiers P.not.not ∧
+                          (∀v: value, dominates' Q' Q₂ (σ[x↦v]))))),
+  by unfold1 dominates',
+  have dominates' P P.not.not σ, from this.symm ▸ h3,
+  show dominates σ P.not.not P, from this
+
+lemma dominates_of_not_not: ∀ {P: prop} {σ: env}, dominates σ P P.not.not
+| P σ :=
+  have h_impl: σ ⊨ vc.implies P.instantiated_n P.not.not.instantiated_n, from valid_env.mpr (
+    assume : σ ⊨ P.instantiated_n,
+    have h1: σ ⊨ P.instantiated_n.not.not, from valid_env.neg_neg.mpr this,
+    have P.not.instantiated = P.instantiated_n.not, from not_dist_instantiated,
+    have h2: σ ⊨ P.not.instantiated.not, from this.symm ▸ h1,
+    have P.not.not.instantiated_n = P.not.instantiated.not, from not_dist_instantiated_n,
+    show σ ⊨ P.not.not.instantiated_n, from this.symm ▸ h2
+  ),
+  have h_calls: calls_env σ P = calls_env σ P.not.not, from set.eq_of_subset_of_subset (
+    assume c: calltrigger,
+    assume : c ∈ calls_env σ P,
+    have c ∈ calls_n_env σ P.not, from prop.has_call_env.not this,
+    show c ∈ calls_env σ P.not.not, from prop.has_call_n_env.not this
+  )
+  (
+    assume c: calltrigger,
+    assume : c ∈ calls_env σ P.not.not,
+    have c ∈ calls_n_env σ P.not, from prop.has_call_env.not.inv this,
+    show c ∈ calls_env σ P, from prop.has_call_n_env.not.inv this
+  ),
+  have h_quantifiers:
+    (∀(t': term) (x: var) (Q₁: prop) (h: callquantifier.mk t' x Q₁ ∈ quantifiers P.not.not),
+                          have Q₁.size < P.not.not.size, from quantifiers_smaller_than_prop.left h,
+    ∃(t: term) (Q₂: prop), callquantifier.mk t x Q₂ ∈ quantifiers P ∧
+                          (∀v: value, dominates' Q₁ Q₂ (σ[x↦v]))), from (
+    assume (t₁: term) (x:var) (Q₁: prop),
+    assume h: callquantifier.mk t₁ x Q₁ ∈ quantifiers P.not.not,
+    have callquantifier.mk t₁ x Q₁ ∈ quantifiers_n P.not, from prop.has_quantifier.not.inv h,
+    have h2: callquantifier.mk t₁ x Q₁ ∈ quantifiers P, from prop.has_quantifier_n.not.inv this,
+    have Q₁.size < P.size, from quantifiers_smaller_than_prop.left h2,
+    have (∀v: value, dominates' Q₁ Q₁ (σ[x↦v])), from (
+      assume v: value,
+      dominates_self
+    ),
+    exists.intro t₁ (exists.intro Q₁ ⟨h2, this⟩)
+  ),
+  have h3: 
+    ((σ ⊨ vc.implies P.instantiated_n P.not.not.instantiated_n) ∧
+    (calls_env σ P = calls_env σ P.not.not) ∧
+    (∀(t': term) (x: var) (Q': prop) (h: callquantifier.mk t' x Q' ∈ quantifiers P.not.not),
+                          have Q'.size < P.not.not.size, from quantifiers_smaller_than_prop.left h,
+    ∃(t: term) (Q₂: prop), callquantifier.mk t x Q₂ ∈ quantifiers P ∧
+                          (∀v: value, dominates' Q' Q₂ (σ[x↦v])))),
+  from ⟨h_impl, ⟨h_calls, h_quantifiers⟩⟩,
+  have
+    dominates' P.not.not P σ = (
+    ((σ ⊨ vc.implies P.instantiated_n P.not.not.instantiated_n) ∧
+    (calls_env σ P = calls_env σ P.not.not) ∧
+    (∀(t': term) (x: var) (Q': prop) (h: callquantifier.mk t' x Q' ∈ quantifiers P.not.not),
+                          have Q'.size < P.not.not.size, from quantifiers_smaller_than_prop.left h,
+    ∃(t: term) (Q₂: prop), callquantifier.mk t x Q₂ ∈ quantifiers P ∧
+                          (∀v: value, dominates' Q' Q₂ (σ[x↦v]))))),
+  by unfold1 dominates',
+  have dominates' P.not.not P σ, from this.symm ▸ h3,
+  show dominates σ P P.not.not, from this
+
+lemma strengthen_impl_with_dominating_instantiations {σ: env} {P P' Q: prop}:
+  dominates σ P' P → σ ⊨ vc.implies (prop.implies P Q).instantiated (prop.implies P' Q).instantiated :=
+  assume P'_dominates_P: dominates σ P' P,
+  show σ ⊨ vc.implies (prop.implies P Q).instantiated (prop.implies P' Q).instantiated, from valid_env.mpr (
+    assume : σ ⊨ (P.not ⋁ Q).instantiated,
+    have h1: σ ⊨ (P.not ⋁ Q).instantiated.not.not, from valid_env.neg_neg.mpr this,
+    have (P.not ⋁ Q).not.instantiated_n = (P.not ⋁ Q).instantiated.not, from not_dist_instantiated_n,
+    have h2: σ ⊨ (P.not ⋁ Q).not.instantiated_n.not, from this.symm ▸ h1,
+    have h3: σ ⊨ vc.implies (P'.not ⋁ Q).not.instantiated_n (P.not ⋁ Q).not.instantiated_n, from valid_env.mpr (
+      assume : σ ⊨ (P'.not ⋁ Q).not.instantiated_n,
+      have h4: σ ⊨ (P'.not.not ⋀ Q.not).instantiated_n, from valid_env.and_not_dist_with_instantiations.mp this,
+      have dominates σ P'.not.not P', from dominates_not_not,
+      have σ ⊨ vc.implies (P'.not.not ⋀ Q.not).instantiated_n (P' ⋀ Q.not).instantiated_n,
+      from valid_env.strengthen_and_with_dominating_instantiations this,
+      have h5: σ ⊨ (P' ⋀ Q.not).instantiated_n, from valid_env.mp this h4,
+      have σ ⊨ vc.implies (P' ⋀ Q.not).instantiated_n (P ⋀ Q.not).instantiated_n,
+      from valid_env.strengthen_and_with_dominating_instantiations P'_dominates_P,
+      have h6: σ ⊨ (P ⋀ Q.not).instantiated_n, from valid_env.mp this h5,
+      have dominates σ P P.not.not, from dominates_of_not_not,
+      have σ ⊨ vc.implies (P ⋀ Q.not).instantiated_n (P.not.not ⋀ Q.not).instantiated_n,
+      from valid_env.strengthen_and_with_dominating_instantiations this,
+      have σ ⊨ (P.not.not ⋀ Q.not).instantiated_n, from valid_env.mp this h6,
+      show σ ⊨ (P.not ⋁ Q).not.instantiated_n, from valid_env.and_not_dist_with_instantiations.mpr this
+    ),
+    have h9: σ ⊨ (P'.not ⋁ Q).not.instantiated_n.not, from valid_env.mt h3 h2,
+    have (P'.not ⋁ Q).not.instantiated_n = (P'.not ⋁ Q).instantiated.not, from not_dist_instantiated_n,
+    have σ ⊨ (P'.not ⋁ Q).instantiated.not.not, from this ▸ h9,
+    show σ ⊨ (P'.not ⋁ Q).instantiated, from valid_env.neg_neg.mp this
   )
 
-lemma dominates_and_left {P P' Q: prop}:
-      (∀σ, dominates σ P' P) → (∀σ, dominates σ (P' ⋀ Q) (P ⋀ Q)) :=
-  assume h: ∀σ, dominates σ P' P,
-  assume σ: env,
-  have calls_env σ P' = calls_env σ P, from (h σ).left,
-  have h_calls: calls_env σ (P' ⋀ Q) = calls_env σ (P ⋀ Q), from same_calls_and_left this,
-  have qualifiers_dominate σ P' P, from (h σ).right.left,
-  have h_quantifiers: qualifiers_dominate σ (P' ⋀ Q) (P ⋀ Q), from same_quantifiers_and_left this,
-  have σ ⊨ vc.implies P'.instantiated_n P.instantiated_n, from (h σ).right.right,
-  have h_impl: σ ⊨ vc.implies (P' ⋀ Q).instantiated_n (P ⋀ Q).instantiated_n,
-  from valid_env.strengthen_and_with_dominating_instantiations (h σ),
-  ⟨h_calls, ⟨h_quantifiers, h_impl⟩⟩
+lemma strengthen_vc {P P' Q S: prop} {σ: env}:
+  dominates σ P' P → (σ ⊨ (prop.implies (P ⋀ Q) S).instantiated) → σ ⊨ (prop.implies (P' ⋀ Q) S).instantiated :=
+  assume : dominates σ P' P,
+  have dominates σ (P' ⋀ Q) (P ⋀ Q), from dominates_and_left this,
+  valid_env.mp (strengthen_impl_with_dominating_instantiations this)
 
-lemma strengthen_pre_exp {P: prop} {Q: propctx} {e: exp}:
+lemma strengthen_exp {P: prop} {Q: propctx} {e: exp}:
       (P ⊢ e : Q) → ∀P': prop, (FV P' = FV P) → (∀σ, dominates σ P' P) → (P' ⊢ e: Q) :=
   assume e_verified: (P ⊢ e : Q),
   begin
@@ -109,7 +329,7 @@ lemma strengthen_pre_exp {P: prop} {Q: propctx} {e: exp}:
       have h1: FV (P' ⋀ (x ≡ value.true)) = FV (P ⋀ (x ≡ value.true)),
       from same_free_and_left free_P'_P,
       have h2: (∀σ, dominates σ (P' ⋀ (x ≡ value.true)) (P ⋀ (x ≡ value.true))),
-      from dominates_and_left P'_dominates_P,
+      from (λσ, dominates_and_left (P'_dominates_P σ)),
       have e'_verified': P' ⋀ (x ≡ value.true) ⊢ e': Q, from ih (P' ⋀ (x ≡ value.true)) h1 h2,
       have x_not_free_in_P': x ∉ FV P', from free_P'_P.symm ▸ x_not_free_in_P,
       show P' ⊢ lett x = true in e' : propctx.exis x ((x ≡ value.true) ⋀ Q),
@@ -123,7 +343,7 @@ lemma strengthen_pre_exp {P: prop} {Q: propctx} {e: exp}:
       have h1: FV (P' ⋀ (x ≡ value.false)) = FV (P ⋀ (x ≡ value.false)),
       from same_free_and_left free_P'_P,
       have h2: (∀σ, dominates σ (P' ⋀ (x ≡ value.false)) (P ⋀ (x ≡ value.false))),
-      from dominates_and_left P'_dominates_P,
+      from (λσ, dominates_and_left (P'_dominates_P σ)),
       have e'_verified': P' ⋀ (x ≡ value.false) ⊢ e': Q, from ih (P' ⋀ (x ≡ value.false)) h1 h2,
       have x_not_free_in_P': x ∉ FV P', from free_P'_P.symm ▸ x_not_free_in_P,
       show P' ⊢ letf x = false in e' : propctx.exis x ((x ≡ value.false) ⋀ Q),
@@ -137,7 +357,7 @@ lemma strengthen_pre_exp {P: prop} {Q: propctx} {e: exp}:
       have h1: FV (P' ⋀ (x ≡ value.num n)) = FV (P ⋀ (x ≡ value.num n)),
       from same_free_and_left free_P'_P,
       have h2: (∀σ, dominates σ (P' ⋀ (x ≡ value.num n)) (P ⋀ (x ≡ value.num n))),
-      from dominates_and_left P'_dominates_P,
+      from (λσ, dominates_and_left (P'_dominates_P σ)),
       have e'_verified': P' ⋀ (x ≡ value.num n) ⊢ e': Q, from ih (P' ⋀ (x ≡ value.num n)) h1 h2,
       have x_not_free_in_P': x ∉ FV P', from free_P'_P.symm ▸ x_not_free_in_P,
       show P' ⊢ letn x = n in e' : propctx.exis x ((x ≡ value.num n) ⋀ Q),
@@ -157,7 +377,7 @@ lemma strengthen_pre_exp {P: prop} {Q: propctx} {e: exp}:
       have h1: FV (P' ⋀ ((spec.func f x R S) ⋀ R)) = FV (P ⋀ ((spec.func f x R S) ⋀ R)),
       from same_free_and_left free_P'_P,
       have h2: (∀σ, dominates σ (P' ⋀ (spec.func f x R S) ⋀ R) (P ⋀ (spec.func f x R S) ⋀ R)),
-      from dominates_and_left P'_dominates_P,
+      from (λσ, dominates_and_left (P'_dominates_P σ)),
       have e₁_verified': P' ⋀ (spec.func f x R S) ⋀ R ⊢ e₁ : Q₁,
       from ih₁ (P' ⋀ (spec.func f x R S) ⋀ R) h1 h2,
 
@@ -166,37 +386,121 @@ lemma strengthen_pre_exp {P: prop} {Q: propctx} {e: exp}:
       from same_free_and_left free_P'_P,
       have h4: (∀σ, dominates σ (P' ⋀ (prop.func f x R (Q₁ (term.app ↑f ↑x) ⋀ ↑S)))
                                 (P ⋀ (prop.func f x R (Q₁ (term.app ↑f ↑x) ⋀ ↑S)))),
-      from dominates_and_left P'_dominates_P,
+      from (λσ, dominates_and_left (P'_dominates_P σ)),
       have e₂_verified': P' ⋀ (prop.func f x R (Q₁ (term.app ↑f ↑x) ⋀ ↑S)) ⊢ e₂ : Q₂,
       from ih₂ (P' ⋀ (prop.func f x R (Q₁ (term.app ↑f ↑x) ⋀ ↑S))) h3 h4,
 
       have func_vc': ∀ (σ : env),
              σ ⊨ prop.instantiated (prop.implies (P' ⋀ ↑(spec.func ↑f x R S) ⋀ R ⋀ Q₁ (term.app ↑f ↑x)) ↑S),
-      from (
-        assume σ: env,
-
-        have dominates σ (prop.or (P' ⋀ ↑(spec.func ↑f x R S) ⋀ R ⋀ Q₁ (term.app ↑f ↑x)).not
-        
-         ↑S).instantiated,
-
-
-        show σ ⊨ (prop.or (P' ⋀ ↑(spec.func ↑f x R S) ⋀ R ⋀ Q₁ (term.app ↑f ↑x)).not ↑S).instantiated,
-        from sorry
-      ),
+      from (λσ, strengthen_vc (P'_dominates_P σ) (func_vc σ)),
 
       show P' ⊢ letf f[x] req R ens S {e₁} in e₂ : propctx.exis f (prop.func f x R (Q₁ (term.app ↑f ↑x) ⋀ ↑S) ⋀ Q₂),
       from exp.vcgen.func f_not_free_in_P' x_not_free_in_P' f_neq_x fv_R' fv_S' e₁_verified'
            e₂_verified' func_vc'
     },
-    case exp.vcgen.unop op x y e' Q' x_free_in_P _ e'_verified vc_valid { from
+    case exp.vcgen.unop op x y P e' Q' x_free_in_P y_not_free_in_P e'_verified vc_valid ih { from
+      assume P': prop,
+      assume free_P'_P: FV P' = FV P,
+      assume P'_dominates_P: (∀σ, dominates σ P' P),
+
+      have x_free_in_P': x ∈ FV P', from free_P'_P.symm ▸ x_free_in_P,
+      have y_not_free_in_P': y ∉ FV P', from free_P'_P.symm ▸ y_not_free_in_P,
+
+      have h1: FV (P' ⋀ y ≡ term.unop op x) = FV (P ⋀ y ≡ term.unop op x),
+      from same_free_and_left free_P'_P,
+      have h2: (∀σ, dominates σ (P' ⋀ y ≡ term.unop op x) (P ⋀ y ≡ term.unop op x)),
+      from (λσ, dominates_and_left (P'_dominates_P σ)),
+      have e'_verified': P' ⋀ y ≡ term.unop op x ⊢ e' : Q',
+      from ih (P' ⋀ y ≡ term.unop op x) h1 h2,
+
+      have vc_valid': ∀ (σ : env),
+             σ ⊨ prop.instantiated (prop.implies P' (prop.pre₁ op x)),
+      from (λσ, valid_env.mp (strengthen_impl_with_dominating_instantiations (P'_dominates_P σ)) (vc_valid σ)),
+
+      show P' ⊢ letop y = op [x] in e' : propctx.exis y (y ≡ term.unop op x ⋀ Q'),
+      from exp.vcgen.unop x_free_in_P' y_not_free_in_P' e'_verified' vc_valid'
     },
-    case exp.vcgen.binop op x y z e' Q' x_free_in_P y_free_in_P _ e'_verified vc_valid { from
+    case exp.vcgen.binop op x y z e' P Q' x_free_in_P y_free_in_P z_not_free_in_P e'_verified vc_valid ih { from
+      assume P': prop,
+      assume free_P'_P: FV P' = FV P,
+      assume P'_dominates_P: (∀σ, dominates σ P' P),
+
+      have x_free_in_P': x ∈ FV P', from free_P'_P.symm ▸ x_free_in_P,
+      have y_free_in_P': y ∈ FV P', from free_P'_P.symm ▸ y_free_in_P,
+      have z_not_free_in_P': z ∉ FV P', from free_P'_P.symm ▸ z_not_free_in_P,
+
+      have h1: FV (P' ⋀ z ≡ term.binop op x y) = FV (P ⋀ z ≡ term.binop op x y),
+      from same_free_and_left free_P'_P,
+      have h2: (∀σ, dominates σ (P' ⋀ z ≡ term.binop op x y) (P ⋀ z ≡ term.binop op x y)),
+      from (λσ, dominates_and_left (P'_dominates_P σ)),
+      have e'_verified': P' ⋀ z ≡ term.binop op x y ⊢ e' : Q',
+      from ih (P' ⋀ z ≡ term.binop op x y) h1 h2,
+
+      have vc_valid': ∀ (σ : env),
+             σ ⊨ prop.instantiated (prop.implies P' (prop.pre₂ op x y)),
+      from (λσ, valid_env.mp (strengthen_impl_with_dominating_instantiations (P'_dominates_P σ)) (vc_valid σ)),
+
+      show P' ⊢ letop2 z = op [x, y] in e' : propctx.exis z (z ≡ term.binop op x y ⋀ Q'),
+      from exp.vcgen.binop x_free_in_P' y_free_in_P' z_not_free_in_P' e'_verified' vc_valid'
     },
-    case exp.vcgen.app y f x e' Q' f_free_in_P x_free_in_P _ e'_verified vc_valid { from
+    case exp.vcgen.app y f x e' P Q' f_free_in_P x_free_in_P y_not_free_in_P e'_verified vc_valid ih { from
+      assume P': prop,
+      assume free_P'_P: FV P' = FV P,
+      assume P'_dominates_P: (∀σ, dominates σ P' P),
+
+      have f_free_in_P': f ∈ FV P', from free_P'_P.symm ▸ f_free_in_P,
+      have x_free_in_P': x ∈ FV P', from free_P'_P.symm ▸ x_free_in_P,
+      have y_not_free_in_P': y ∉ FV P', from free_P'_P.symm ▸ y_not_free_in_P,
+
+      have h1: FV (P' ⋀ prop.call f x ⋀ prop.post f x ⋀ y ≡ term.app f x)
+             = FV (P ⋀ prop.call f x ⋀ prop.post f x ⋀ y ≡ term.app f x),
+      from same_free_and_left free_P'_P,
+
+      have h2: (∀σ, dominates σ (P' ⋀ prop.call f x ⋀ prop.post f x ⋀ y ≡ term.app f x)
+                                (P ⋀ prop.call f x ⋀ prop.post f x ⋀ y ≡ term.app f x)),
+      from (λσ, dominates_and_left (P'_dominates_P σ)),
+
+      have e'_verified': P' ⋀ prop.call f x ⋀ prop.post f x ⋀ y ≡ term.app f x ⊢ e' : Q',
+      from ih (P' ⋀ prop.call f x ⋀ prop.post f x ⋀ y ≡ term.app f x) h1 h2,
+
+      have vc_valid': ∀ (σ : env),
+             σ ⊨ prop.instantiated (prop.implies (P' ⋀ prop.call f x) (term.unop unop.isFunc f ⋀ prop.pre f x)),
+      from (λσ, strengthen_vc (P'_dominates_P σ) (vc_valid σ)),
+
+      show P' ⊢ letapp y = f [x] in e' : propctx.exis y (prop.call f x ⋀ prop.post f x ⋀ y ≡ term.app f x ⋀ Q'),
+      from exp.vcgen.app f_free_in_P' x_free_in_P' y_not_free_in_P' e'_verified' vc_valid'
     },
-    case exp.vcgen.ite x e₂ e₁ Q₁ Q₂ x_free_in_P _ _ vc_valid { from
+    case exp.vcgen.ite x e₂ e₁ P Q₁ Q₂ x_free_in_P e₁_verified e₂_verified vc_valid ih₁ ih₂ { from
+      assume P': prop,
+      assume free_P'_P: FV P' = FV P,
+      assume P'_dominates_P: (∀σ, dominates σ P' P),
+
+      have x_free_in_P': x ∈ FV P', from free_P'_P.symm ▸ x_free_in_P,
+
+      have h1: FV (P' ⋀ x) = FV (P ⋀ x), from same_free_and_left free_P'_P,
+      have h2: (∀σ, dominates σ (P' ⋀ x) (P ⋀ x)), from (λσ, dominates_and_left (P'_dominates_P σ)),
+      have e₁_verified': P' ⋀ x ⊢ e₁ : Q₁, from ih₁ (P' ⋀ x) h1 h2,
+
+      have h1: FV (P' ⋀ term.unop unop.not x) = FV (P ⋀ term.unop unop.not x), from same_free_and_left free_P'_P,
+      have h2: (∀σ, dominates σ (P' ⋀ term.unop unop.not x) (P ⋀ term.unop unop.not x)),
+      from (λσ, dominates_and_left (P'_dominates_P σ)),
+      have e₂_verified': P' ⋀ term.unop unop.not x ⊢ e₂ : Q₂, from ih₂ (P' ⋀ term.unop unop.not x) h1 h2,
+
+      have vc_valid': ∀ (σ : env),
+             σ ⊨ prop.instantiated (prop.implies P' (term.unop unop.isBool x)),
+      from (λσ, valid_env.mp (strengthen_impl_with_dominating_instantiations (P'_dominates_P σ)) (vc_valid σ)),
+
+      show P' ⊢ exp.ite x e₁ e₂ : propctx.implies x Q₁ ⋀ propctx.implies (term.unop unop.not x) Q₂,
+      from exp.vcgen.ite x_free_in_P' e₁_verified' e₂_verified' vc_valid'
     },
-    case exp.vcgen.return x x_free_in_P { from
+    case exp.vcgen.return x P x_free_in_P { from
+      assume P': prop,
+      assume free_P'_P: FV P' = FV P,
+      assume P'_dominates_P: (∀σ, dominates σ P' P),
+
+      have x_free_in_P': x ∈ FV P', from free_P'_P.symm ▸ x_free_in_P,
+
+      show P' ⊢ exp.return x : (x ≣ •), from exp.vcgen.return x_free_in_P'
     }
   end
 
