soundness.lean
@@ -3,9 +3,9 @@ import data.set
 import .syntax .notations .logic .evaluation .vcgen .progress .preservation
 
 lemma trivial_precondition:
-  ∀σ, σ ⊨ vc.implies (prop.instantiated_n (value.true && value.true)) (prop.instantiated_n (value.true)) :=
+  ∀σ, σ ⊨ vc.implies (prop.instantiated_n (value.true ⋀ value.true)) (prop.instantiated_n (value.true)) :=
   assume σ: env,
-  show σ ⊨ vc.implies (prop.instantiated_n (value.true && value.true)) (prop.instantiated_n (value.true)),
+  show σ ⊨ vc.implies (prop.instantiated_n (value.true ⋀ value.true)) (prop.instantiated_n (value.true)),
   from valid_env.mpr (
     assume _,
     have h: σ ⊨ value.true, from valid_env.true,
@@ -15,10 +15,10 @@ lemma trivial_precondition:
     show σ ⊨ (prop.instantiated_n (value.true)), from valid_env.instantiated_n_of_instantiated this
   )
 
-lemma trivial_freevars: FV (prop.term value.true && prop.term value.true) = FV (prop.term value.true) :=
-  have h1: FV (prop.term value.true && prop.term value.true) = ∅, from set.eq_empty_of_forall_not_mem (
+lemma trivial_freevars: FV (prop.term value.true ⋀ prop.term value.true) = FV (prop.term value.true) :=
+  have h1: FV (prop.term value.true ⋀ prop.term value.true) = ∅, from set.eq_empty_of_forall_not_mem (
     assume x: var,
-    assume : x ∈ FV (prop.term value.true && prop.term value.true),
+    assume : x ∈ FV (prop.term value.true ⋀ prop.term value.true),
     have x ∈ FV (prop.term value.true) ∨ x ∈ FV (prop.term value.true), from free_in_prop.and.inv this,
     or.elim this (
       assume : x ∈ FV (prop.term value.true),
@@ -36,12 +36,12 @@ lemma trivial_freevars: FV (prop.term value.true && prop.term value.true) = FV (
     have x ∈ FV (term.value value.true), from free_in_prop.term.inv this,
     show «false», from free_in_term.value.inv this
   ),
-  show FV (prop.term value.true && prop.term value.true) = FV (prop.term value.true), from eq.trans h1 h2.symm
+  show FV (prop.term value.true ⋀ prop.term value.true) = FV (prop.term value.true), from eq.trans h1 h2.symm
 
-lemma trivial_calls: calls (prop.term value.true && prop.term value.true) = calls (prop.term value.true) :=
-  have h1: calls (prop.term value.true && prop.term value.true) = ∅, from set.eq_empty_of_forall_not_mem (
+lemma trivial_calls: calls (prop.term value.true ⋀ prop.term value.true) = calls (prop.term value.true) :=
+  have h1: calls (prop.term value.true ⋀ prop.term value.true) = ∅, from set.eq_empty_of_forall_not_mem (
     assume c: calltrigger,
-    assume : c ∈ calls (prop.term value.true && prop.term value.true),
+    assume : c ∈ calls (prop.term value.true ⋀ prop.term value.true),
     have c ∈ calls (prop.term value.true) ∨ c ∈ calls (prop.term value.true), from has_call.and.inv this,
     or.elim this (
       assume : c ∈ calls (prop.term value.true),
@@ -56,12 +56,12 @@ lemma trivial_calls: calls (prop.term value.true && prop.term value.true) = call
     assume : c ∈ calls (prop.term value.true),
     show «false», from has_call.term.inv this
   ),
-  show calls (prop.term value.true && prop.term value.true) = calls (prop.term value.true), from eq.trans h1 h2.symm
+  show calls (prop.term value.true ⋀ prop.term value.true) = calls (prop.term value.true), from eq.trans h1 h2.symm
 
-lemma trivial_quantifiers: quantifiers (prop.term value.true && prop.term value.true) = quantifiers (prop.term value.true) :=
-  have h1: quantifiers (prop.term value.true && prop.term value.true) = ∅, from set.eq_empty_of_forall_not_mem (
+lemma trivial_quantifiers: quantifiers (prop.term value.true ⋀ prop.term value.true) = quantifiers (prop.term value.true) :=
+  have h1: quantifiers (prop.term value.true ⋀ prop.term value.true) = ∅, from set.eq_empty_of_forall_not_mem (
     assume q: callquantifier,
-    assume : q ∈ quantifiers (prop.term value.true && prop.term value.true),
+    assume : q ∈ quantifiers (prop.term value.true ⋀ prop.term value.true),
     have q ∈ quantifiers (prop.term value.true) ∨ q ∈ quantifiers (prop.term value.true), from has_quantifier.and.inv this,
     or.elim this (
       assume : q ∈ quantifiers (prop.term value.true),
@@ -76,7 +76,7 @@ lemma trivial_quantifiers: quantifiers (prop.term value.true && prop.term value.
     assume : q ∈ quantifiers (prop.term value.true),
     show «false», from has_quantifier.term.inv this
   ),
-  show quantifiers (prop.term value.true && prop.term value.true) = quantifiers (prop.term value.true), from eq.trans h1 h2.symm
+  show quantifiers (prop.term value.true ⋀ prop.term value.true) = quantifiers (prop.term value.true), from eq.trans h1 h2.symm
 
 lemma soundness {s s': stack}: (s ⟶* s') → ∀H, (H ⊢ₛ s) → (is_value s' ∨ ∃h s'', s' ⟶ h, s'') :=
   assume steps_to_s': s ⟶* s',
@@ -100,8 +100,8 @@ theorem soundness_source_programs {e: exp} {s: stack} {Q: propctx}:
 
   assume initial_verified: value.true ⊢ e: Q,
   assume steps_to_s: (env.empty, e) ⟶* s,
-  have (prop.term value.true && prop.term value.true) ⊢ e: Q,
-  from strengthen_pre_exp initial_verified (prop.term value.true && prop.term value.true)
+  have (prop.term value.true ⋀ prop.term value.true) ⊢ e: Q,
+  from strengthen_pre_exp initial_verified (prop.term value.true ⋀ prop.term value.true)
        trivial_freevars trivial_calls trivial_quantifiers trivial_precondition,
   have list.nil ⊢ₛ (env.empty, e), from stack.vcgen.top env.vcgen.empty this,
   show is_value s ∨ ∃h s', s ⟶ h, s', from soundness steps_to_s list.nil this
